Source/Dafny/Parser.cs
@@ -1704,7 +1704,7 @@ int StringToInt(string s, int defaultValue, string errString) {
 			while (la.kind == 72) {
 				Attribute(ref attrs);
 			}
-			NoUSIdent(out id);
+			FuMe_Ident(out id);
 			if (la.kind == 76 || la.kind == 78) {
 				if (la.kind == 78) {
 					GenericParameters(typeArgs, false);
@@ -1782,7 +1782,7 @@ int StringToInt(string s, int defaultValue, string errString) {
 			while (la.kind == 72) {
 				Attribute(ref attrs);
 			}
-			NoUSIdent(out id);
+			FuMe_Ident(out id);
 			if (la.kind == 74 || la.kind == 76 || la.kind == 78) {
 				if (la.kind == 78) {
 					GenericParameters(typeArgs, false);
@@ -1964,8 +1964,8 @@ int StringToInt(string s, int defaultValue, string errString) {
 		while (la.kind == 72) {
 			Attribute(ref attrs);
 		}
-		if (la.kind == 1) {
-			NoUSIdent(out id);
+		if (la.kind == 1 || la.kind == 2) {
+			FuMe_Ident(out id);
 			hasName = true; 
 		}
 		if (!hasName) {
@@ -2394,8 +2394,8 @@ int StringToInt(string s, int defaultValue, string errString) {
 			tok = t; 
 			while (la.kind == 30) {
 				Get();
-				Expect(1);
-				tok = t; List<Type> typeArgs; 
+				TypeNameOrCtorSuffix(out tok);
+				List<Type> typeArgs; 
 				OptGenericInstantiation(out typeArgs, inExpressionContext);
 				e = new ExprDotName(tok, e, tok.val, typeArgs); 
 			}
@@ -2589,6 +2589,16 @@ ref Attributes readsAttrs, ref Attributes modAttrs, ref Attributes decrAttrs) {
 		} else SynErr(196);
 	}
 
+	void FuMe_Ident(out IToken id) {
+		id = Token.NoToken; 
+		if (la.kind == 1) {
+			NoUSIdent(out id);
+		} else if (la.kind == 2) {
+			Get();
+			id = t; 
+		} else SynErr(197);
+	}
+
 	void KType(ref FixpointPredicate.KType kType) {
 		Expect(74);
 		if (la.kind == 10) {
@@ -2597,7 +2607,7 @@ ref Attributes readsAttrs, ref Attributes modAttrs, ref Attributes decrAttrs) {
 		} else if (la.kind == 12) {
 			Get();
 			kType = FixpointPredicate.KType.ORDINAL; 
-		} else SynErr(197);
+		} else SynErr(198);
 		Expect(75);
 	}
 
@@ -2609,7 +2619,7 @@ List<Expression> decreases, ref Attributes decAttrs, ref Attributes modAttrs, st
 		Contract.Requires(cce.NonNullElements(decreases));
 		Expression e;  FrameExpression fe;  bool isFree = false; Attributes ensAttrs = null; Attributes reqAttrs = null;
 		
-		while (!(StartOf(19))) {SynErr(198); Get();}
+		while (!(StartOf(19))) {SynErr(199); Get();}
 		if (la.kind == 66) {
 			Get();
 			while (IsAttribute()) {
@@ -2646,7 +2656,7 @@ List<Expression> decreases, ref Attributes decAttrs, ref Attributes modAttrs, st
 				Expression(out e, false, false);
 				OldSemi();
 				ens.Add(new MaybeFreeExpression(e, isFree, ensAttrs)); 
-			} else SynErr(199);
+			} else SynErr(200);
 		} else if (la.kind == 42) {
 			Get();
 			while (IsAttribute()) {
@@ -2654,7 +2664,7 @@ List<Expression> decreases, ref Attributes decAttrs, ref Attributes modAttrs, st
 			}
 			DecreasesList(decreases, true, false);
 			OldSemi();
-		} else SynErr(200);
+		} else SynErr(201);
 	}
 
 	void DividedBlockStmt(out DividedBlockStmt body, out IToken bodyStart, out IToken bodyEnd) {
@@ -2702,7 +2712,7 @@ List<Expression> decreases, ref Attributes decAttrs, ref Attributes modAttrs, st
 			Ident(out id);
 			fieldName = id.val; 
 			fe = new FrameExpression(id, new ImplicitThisExpr(id), fieldName); 
-		} else SynErr(201);
+		} else SynErr(202);
 	}
 
 	void DecreasesList(List<Expression> decreases, bool allowWildcard, bool allowLambda) {
@@ -2742,6 +2752,17 @@ List<Expression> decreases, ref Attributes decAttrs, ref Attributes modAttrs, st
 		
 	}
 
+	void TypeNameOrCtorSuffix(out IToken id) {
+		id = Token.NoToken; 
+		if (la.kind == 1) {
+			Get();
+			id = t; 
+		} else if (la.kind == 2) {
+			Get();
+			id = t; 
+		} else SynErr(203);
+	}
+
 	void GenericInstantiation(List<Type> gt) {
 		Contract.Requires(cce.NonNullElements(gt)); Type/*!*/ ty; 
 		Expect(78);
@@ -2761,7 +2782,7 @@ List<Expression> decreases, ref Attributes decAttrs, ref Attributes modAttrs, st
 		Contract.Requires(decreases == null || cce.NonNullElements(decreases));
 		Expression/*!*/ e;  FrameExpression/*!*/ fe;
 		Attributes ensAttrs = null; Attributes reqAttrs = null; 
-		while (!(StartOf(20))) {SynErr(202); Get();}
+		while (!(StartOf(20))) {SynErr(204); Get();}
 		if (la.kind == 68) {
 			Get();
 			while (IsAttribute()) {
@@ -2797,7 +2818,7 @@ List<Expression> decreases, ref Attributes decAttrs, ref Attributes modAttrs, st
 			
 			DecreasesList(decreases, false, false);
 			OldSemi();
-		} else SynErr(203);
+		} else SynErr(205);
 	}
 
 	void FunctionBody(out Expression/*!*/ e, out IToken bodyStart, out IToken bodyEnd) {
@@ -2816,7 +2837,7 @@ List<Expression> decreases, ref Attributes decAttrs, ref Attributes modAttrs, st
 			fe = new FrameExpression(t, new WildcardExpr(t), null); 
 		} else if (StartOf(21)) {
 			FrameExpression(out fe, allowSemi, false);
-		} else SynErr(204);
+		} else SynErr(206);
 	}
 
 	void PossiblyWildExpression(out Expression e, bool allowLambda) {
@@ -2827,7 +2848,7 @@ List<Expression> decreases, ref Attributes decAttrs, ref Attributes modAttrs, st
 			e = new WildcardExpr(t); 
 		} else if (StartOf(9)) {
 			Expression(out e, false, allowLambda);
-		} else SynErr(205);
+		} else SynErr(207);
 	}
 
 	void Stmt(List<Statement/*!*/>/*!*/ ss) {
@@ -2844,7 +2865,7 @@ List<Expression> decreases, ref Attributes decAttrs, ref Attributes modAttrs, st
 		IToken bodyStart, bodyEnd;
 		int breakCount;
 		
-		while (!(StartOf(22))) {SynErr(206); Get();}
+		while (!(StartOf(22))) {SynErr(208); Get();}
 		switch (la.kind) {
 		case 72: {
 			BlockStmt(out bs, out bodyStart, out bodyEnd);
@@ -2919,8 +2940,8 @@ List<Expression> decreases, ref Attributes decAttrs, ref Attributes modAttrs, st
 					Get();
 					breakCount++; 
 				}
-			} else SynErr(207);
-			while (!(la.kind == 0 || la.kind == 32)) {SynErr(208); Get();}
+			} else SynErr(209);
+			while (!(la.kind == 0 || la.kind == 32)) {SynErr(210); Get();}
 			Expect(32);
 			s = label != null ? new BreakStmt(x, t, label) : new BreakStmt(x, t, breakCount); 
 			break;
@@ -2933,7 +2954,7 @@ List<Expression> decreases, ref Attributes decAttrs, ref Attributes modAttrs, st
 			SkeletonStmt(out s);
 			break;
 		}
-		default: SynErr(209); break;
+		default: SynErr(211); break;
 		}
 	}
 
@@ -2956,12 +2977,12 @@ List<Expression> decreases, ref Attributes decAttrs, ref Attributes modAttrs, st
 				BlockStmt(out proof, out proofStart, out proofEnd);
 			} else if (la.kind == 32) {
 				Get();
-			} else SynErr(210);
+			} else SynErr(212);
 		} else if (la.kind == 85) {
 			Get();
 			dotdotdot = t; 
 			Expect(32);
-		} else SynErr(211);
+		} else SynErr(213);
 		if (dotdotdot != null) {
 		 s = new SkeletonStatement(new AssertStmt(x, t, new LiteralExpr(x, true), null, attrs), dotdotdot, null);
 		} else {
@@ -2985,7 +3006,7 @@ List<Expression> decreases, ref Attributes decAttrs, ref Attributes modAttrs, st
 		} else if (la.kind == 85) {
 			Get();
 			dotdotdot = t; 
-		} else SynErr(212);
+		} else SynErr(214);
 		Expect(32);
 		if (dotdotdot != null) {
 		 s = new SkeletonStatement(new AssumeStmt(x, t, new LiteralExpr(x, true), attrs), dotdotdot, null);
@@ -3066,13 +3087,13 @@ List<Expression> decreases, ref Attributes decAttrs, ref Attributes modAttrs, st
 					suchThatAssume = t; 
 				}
 				Expression(out suchThat, false, true);
-			} else SynErr(213);
+			} else SynErr(215);
 			Expect(32);
 			endTok = t; 
 		} else if (la.kind == 24) {
 			Get();
 			SemErr(t, "invalid statement (did you forget the 'label' keyword?)"); 
-		} else SynErr(214);
+		} else SynErr(216);
 		if (suchThat != null) {
 		 s = new AssignSuchThatStmt(x, endTok, lhss, suchThat, suchThatAssume, null);
 		} else {
@@ -3141,7 +3162,7 @@ List<Expression> decreases, ref Attributes decAttrs, ref Attributes modAttrs, st
 					Expression(out suchThat, false, true);
 				}
 			}
-			while (!(la.kind == 0 || la.kind == 32)) {SynErr(215); Get();}
+			while (!(la.kind == 0 || la.kind == 32)) {SynErr(217); Get();}
 			Expect(32);
 			endTok = t; 
 			ConcreteUpdateStatement update;
@@ -3177,11 +3198,11 @@ List<Expression> decreases, ref Attributes decAttrs, ref Attributes modAttrs, st
 				}
 				Expect(28);
 				SemErr(pat.tok, "LHS of assign-such-that expression must be variables, not general patterns"); 
-			} else SynErr(216);
+			} else SynErr(218);
 			Expression(out e, false, true);
 			Expect(32);
 			s = new LetStmt(e.tok, e.tok, pat, e); 
-		} else SynErr(217);
+		} else SynErr(219);
 	}
 
 	void IfStmt(out Statement/*!*/ ifStmt) {
@@ -3221,7 +3242,7 @@ List<Expression> decreases, ref Attributes decAttrs, ref Attributes modAttrs, st
 				} else if (la.kind == 72) {
 					BlockStmt(out bs, out bodyStart, out bodyEnd);
 					els = bs; endTok = bs.EndTok; 
-				} else SynErr(218);
+				} else SynErr(220);
 			}
 			if (guardEllipsis != null) {
 			 ifStmt = new SkeletonStatement(new IfStmt(x, endTok, isExistentialGuard, guard, thn, els), guardEllipsis, null);
@@ -3229,7 +3250,7 @@ List<Expression> decreases, ref Attributes decAttrs, ref Attributes modAttrs, st
 			 ifStmt = new IfStmt(x, endTok, isExistentialGuard, guard, thn, els);
 			}
 			
-		} else SynErr(219);
+		} else SynErr(221);
 	}
 
 	void WhileStmt(out Statement stmt) {
@@ -3275,7 +3296,7 @@ List<Expression> decreases, ref Attributes decAttrs, ref Attributes modAttrs, st
 				Expect(85);
 				bodyEllipsis = t; endTok = t; isDirtyLoop = false; 
 			} else if (StartOf(26)) {
-			} else SynErr(220);
+			} else SynErr(222);
 			if (guardEllipsis != null || bodyEllipsis != null) {
 			 if (mod != null) {
 			   SemErr(mod[0].E.tok, "'modifies' clauses are not allowed on refining loops");
@@ -3293,7 +3314,7 @@ List<Expression> decreases, ref Attributes decAttrs, ref Attributes modAttrs, st
 			 stmt = new WhileStmt(x, endTok, guard, invariants, new Specification<Expression>(decreases, decAttrs), new Specification<FrameExpression>(mod, modAttrs), body);
 			}
 			
-		} else SynErr(221);
+		} else SynErr(223);
 	}
 
 	void MatchStmt(out Statement/*!*/ s) {
@@ -3318,7 +3339,7 @@ List<Expression> decreases, ref Attributes decAttrs, ref Attributes modAttrs, st
 				CaseStatement(out c);
 				cases.Add(c); 
 			}
-		} else SynErr(222);
+		} else SynErr(224);
 		s = new MatchStmt(x, t, e, cases, usesOptionalBraces); 
 	}
 
@@ -3343,7 +3364,7 @@ List<Expression> decreases, ref Attributes decAttrs, ref Attributes modAttrs, st
 			x = t;
 			errors.Deprecated(t, "the 'parallel' keyword has been deprecated; the comprehension statement now uses the keyword 'forall' (and the parentheses around the bound variables are now optional)");
 			
-		} else SynErr(223);
+		} else SynErr(225);
 		if (la.kind == _openparen) {
 			Expect(76);
 			if (la.kind == 1) {
@@ -3354,7 +3375,7 @@ List<Expression> decreases, ref Attributes decAttrs, ref Attributes modAttrs, st
 			if (la.kind == _ident) {
 				QuantifierDomain(out bvars, out attrs, out range);
 			}
-		} else SynErr(224);
+		} else SynErr(226);
 		if (bvars == null) { bvars = new List<BoundVar>(); }
 		if (range == null) { range = new LiteralExpr(x, true); }
 		
@@ -3443,7 +3464,7 @@ List<Expression> decreases, ref Attributes decAttrs, ref Attributes modAttrs, st
 				} else if (la.kind == 35) {
 					CalcStmt(out subCalc);
 					hintEnd = subCalc.EndTok; subhints.Add(subCalc); 
-				} else SynErr(225);
+				} else SynErr(227);
 			}
 			var h = new BlockStmt(hintStart, hintEnd, subhints); // if the hint is empty, hintStart is the first token of the next line, but it doesn't matter because the block statement is just used as a container
 			hints.Add(h);
@@ -3485,14 +3506,14 @@ List<Expression> decreases, ref Attributes decAttrs, ref Attributes modAttrs, st
 		} else if (la.kind == 85) {
 			Get();
 			ellipsisToken = t; 
-		} else SynErr(226);
+		} else SynErr(228);
 		if (la.kind == 72) {
 			BlockStmt(out body, out bodyStart, out endTok);
 		} else if (la.kind == 32) {
-			while (!(la.kind == 0 || la.kind == 32)) {SynErr(227); Get();}
+			while (!(la.kind == 0 || la.kind == 32)) {SynErr(229); Get();}
 			Get();
 			endTok = t; 
-		} else SynErr(228);
+		} else SynErr(230);
 		s = new ModifyStmt(tok, endTok, mod, attrs, body);
 		if (ellipsisToken != null) {
 		 s = new SkeletonStatement(s, ellipsisToken, null);
@@ -3501,13 +3522,13 @@ List<Expression> decreases, ref Attributes decAttrs, ref Attributes modAttrs, st
 	}
 
 	void LabelIdent(out IToken id) {
-		id = null; /* to please compiler */ 
+		id = Token.NoToken; 
 		if (la.kind == 1) {
-			WildIdent(out id, false);
+			NoUSIdent(out id);
 		} else if (la.kind == 2) {
 			Get();
 			id = t; 
-		} else SynErr(229);
+		} else SynErr(231);
 	}
 
 	void ReturnStmt(out Statement/*!*/ s) {
@@ -3522,7 +3543,7 @@ List<Expression> decreases, ref Attributes decAttrs, ref Attributes modAttrs, st
 		} else if (la.kind == 106) {
 			Get();
 			returnTok = t; isYield = true; 
-		} else SynErr(230);
+		} else SynErr(232);
 		if (StartOf(29)) {
 			Rhs(out r);
 			rhss = new List<AssignmentRhs>(); rhss.Add(r); 
@@ -3606,7 +3627,7 @@ List<Expression> decreases, ref Attributes decAttrs, ref Attributes modAttrs, st
 						Expect(77);
 					}
 				}
-			} else SynErr(231);
+			} else SynErr(233);
 			if (ee != null) {
 			 if (display != null) {
 			   r = new TypeRhs(newToken, ty, ee[0], display);
@@ -3625,7 +3646,7 @@ List<Expression> decreases, ref Attributes decAttrs, ref Attributes modAttrs, st
 		} else if (StartOf(9)) {
 			Expression(out e, false, true);
 			r = new ExprRhs(e); 
-		} else SynErr(232);
+		} else SynErr(234);
 		while (la.kind == 72) {
 			Attribute(ref attrs);
 		}
@@ -3646,7 +3667,7 @@ List<Expression> decreases, ref Attributes decAttrs, ref Attributes modAttrs, st
 			while (la.kind == 30 || la.kind == 74 || la.kind == 76) {
 				Suffix(ref e);
 			}
-		} else SynErr(233);
+		} else SynErr(235);
 	}
 
 	void NewArray(out List<Expression> ee, out Expression arrayElementInit, out List<Expression> display ) {
@@ -3690,7 +3711,7 @@ List<Expression> decreases, ref Attributes decAttrs, ref Attributes modAttrs, st
 					Expect(75);
 				}
 			}
-		} else SynErr(234);
+		} else SynErr(236);
 		if (ee.Count == 0) {
 		 // an error occurred while parsing, but we still want to make sure to return a nonempty "ee"
 		 ee.Add(new LiteralExpr(x, 0));
@@ -3752,7 +3773,7 @@ List<Expression> decreases, ref Attributes decAttrs, ref Attributes modAttrs, st
 			IdentTypeOptional(out bv);
 			pat = new CasePattern(bv.tok, bv);
 			
-		} else SynErr(235);
+		} else SynErr(237);
 		if (pat == null) {
 		 pat = new CasePattern(t, "_ParseError", new List<CasePattern>());
 		}
@@ -3780,7 +3801,7 @@ List<Expression> decreases, ref Attributes decAttrs, ref Attributes modAttrs, st
 				AlternativeBlockCase(allowExistentialGuards, out alt);
 				alternatives.Add(alt); 
 			}
-		} else SynErr(236);
+		} else SynErr(238);
 		endTok = t; 
 	}
 
@@ -3818,7 +3839,7 @@ List<Expression> decreases, ref Attributes decAttrs, ref Attributes modAttrs, st
 		} else if (StartOf(9)) {
 			Expression(out ee, true, true);
 			e = ee; 
-		} else SynErr(237);
+		} else SynErr(239);
 	}
 
 	void AlternativeBlockCase(bool allowExistentialGuards, out GuardedAlternative alt) {
@@ -3833,13 +3854,13 @@ List<Expression> decreases, ref Attributes decAttrs, ref Attributes modAttrs, st
 			isExistentialGuard = true; 
 		} else if (StartOf(9)) {
 			Expression(out e, true, false);
-		} else SynErr(238);
+		} else SynErr(240);
 		Expect(33);
 		body = new List<Statement>(); 
-		while (!(StartOf(31))) {SynErr(239); Get();}
+		while (!(StartOf(31))) {SynErr(241); Get();}
 		while (IsNotEndOfCase()) {
 			Stmt(body);
-			while (!(StartOf(31))) {SynErr(240); Get();}
+			while (!(StartOf(31))) {SynErr(242); Get();}
 		}
 		alt = new GuardedAlternative(x, isExistentialGuard, e, body); 
 	}
@@ -3849,7 +3870,7 @@ List<Expression> decreases, ref Attributes decAttrs, ref Attributes modAttrs, st
 		bool isFree = false; Attributes attrs = null;
 		
 		if (la.kind == 43 || la.kind == 105) {
-			while (!(la.kind == 0 || la.kind == 43 || la.kind == 105)) {SynErr(241); Get();}
+			while (!(la.kind == 0 || la.kind == 43 || la.kind == 105)) {SynErr(243); Get();}
 			if (la.kind == 105) {
 				Get();
 				isFree = true; errors.Deprecated(t, "the 'free' keyword is soon to be deprecated"); 
@@ -3862,7 +3883,7 @@ List<Expression> decreases, ref Attributes decAttrs, ref Attributes modAttrs, st
 			invariants.Add(new MaybeFreeExpression(e, isFree, attrs)); 
 			OldSemi();
 		} else if (la.kind == 42) {
-			while (!(la.kind == 0 || la.kind == 42)) {SynErr(242); Get();}
+			while (!(la.kind == 0 || la.kind == 42)) {SynErr(244); Get();}
 			Get();
 			while (IsAttribute()) {
 				Attribute(ref decAttrs);
@@ -3870,7 +3891,7 @@ List<Expression> decreases, ref Attributes decAttrs, ref Attributes modAttrs, st
 			DecreasesList(decreases, true, true);
 			OldSemi();
 		} else if (la.kind == 66) {
-			while (!(la.kind == 0 || la.kind == 66)) {SynErr(243); Get();}
+			while (!(la.kind == 0 || la.kind == 66)) {SynErr(245); Get();}
 			Get();
 			mod = mod ?? new List<FrameExpression>(); 
 			while (IsAttribute()) {
@@ -3884,7 +3905,7 @@ List<Expression> decreases, ref Attributes decAttrs, ref Attributes modAttrs, st
 				mod.Add(fe); 
 			}
 			OldSemi();
-		} else SynErr(244);
+		} else SynErr(246);
 	}
 
 	void CaseStatement(out MatchCaseStmt/*!*/ c) {
@@ -3923,12 +3944,12 @@ List<Expression> decreases, ref Attributes decAttrs, ref Attributes modAttrs, st
 				arguments.Add(pat); 
 			}
 			Expect(77);
-		} else SynErr(245);
+		} else SynErr(247);
 		Expect(33);
-		while (!(StartOf(31))) {SynErr(246); Get();}
+		while (!(StartOf(31))) {SynErr(248); Get();}
 		while (IsNotEndOfCase()) {
 			Stmt(body);
-			while (!(StartOf(31))) {SynErr(247); Get();}
+			while (!(StartOf(31))) {SynErr(249); Get();}
 		}
 		c = new MatchCaseStmt(x, name, arguments, body); 
 	}
@@ -4027,7 +4048,7 @@ List<Expression> decreases, ref Attributes decAttrs, ref Attributes modAttrs, st
 			x = t;  binOp = BinaryExpr.Opcode.Exp; 
 			break;
 		}
-		default: SynErr(248); break;
+		default: SynErr(250); break;
 		}
 		if (k == null) {
 		 op = new Microsoft.Dafny.CalcStmt.BinaryCalcOp(binOp);
@@ -4042,7 +4063,7 @@ List<Expression> decreases, ref Attributes decAttrs, ref Attributes modAttrs, st
 			Get();
 		} else if (la.kind == 128) {
 			Get();
-		} else SynErr(249);
+		} else SynErr(251);
 	}
 
 	void ImpliesOp() {
@@ -4050,7 +4071,7 @@ List<Expression> decreases, ref Attributes decAttrs, ref Attributes modAttrs, st
 			Get();
 		} else if (la.kind == 130) {
 			Get();
-		} else SynErr(250);
+		} else SynErr(252);
 	}
 
 	void ExpliesOp() {
@@ -4058,7 +4079,7 @@ List<Expression> decreases, ref Attributes decAttrs, ref Attributes modAttrs, st
 			Get();
 		} else if (la.kind == 132) {
 			Get();
-		} else SynErr(251);
+		} else SynErr(253);
 	}
 
 	void AndOp() {
@@ -4066,7 +4087,7 @@ List<Expression> decreases, ref Attributes decAttrs, ref Attributes modAttrs, st
 			Get();
 		} else if (la.kind == 134) {
 			Get();
-		} else SynErr(252);
+		} else SynErr(254);
 	}
 
 	void OrOp() {
@@ -4074,7 +4095,7 @@ List<Expression> decreases, ref Attributes decAttrs, ref Attributes modAttrs, st
 			Get();
 		} else if (la.kind == 136) {
 			Get();
-		} else SynErr(253);
+		} else SynErr(255);
 	}
 
 	void NegOp() {
@@ -4082,7 +4103,7 @@ List<Expression> decreases, ref Attributes decAttrs, ref Attributes modAttrs, st
 			Get();
 		} else if (la.kind == 137) {
 			Get();
-		} else SynErr(254);
+		} else SynErr(256);
 	}
 
 	void Forall() {
@@ -4090,7 +4111,7 @@ List<Expression> decreases, ref Attributes decAttrs, ref Attributes modAttrs, st
 			Get();
 		} else if (la.kind == 138) {
 			Get();
-		} else SynErr(255);
+		} else SynErr(257);
 	}
 
 	void Exists() {
@@ -4098,7 +4119,7 @@ List<Expression> decreases, ref Attributes decAttrs, ref Attributes modAttrs, st
 			Get();
 		} else if (la.kind == 140) {
 			Get();
-		} else SynErr(256);
+		} else SynErr(258);
 	}
 
 	void QSep() {
@@ -4106,7 +4127,7 @@ List<Expression> decreases, ref Attributes decAttrs, ref Attributes modAttrs, st
 			Get();
 		} else if (la.kind == 29) {
 			Get();
-		} else SynErr(257);
+		} else SynErr(259);
 	}
 
 	void EquivExpression(out Expression e0, bool allowSemi, bool allowLambda, bool allowBitwiseOps) {
@@ -4141,7 +4162,7 @@ List<Expression> decreases, ref Attributes decAttrs, ref Attributes modAttrs, st
 					e0 = new BinaryExpr(x, BinaryExpr.Opcode.Exp, e1, e0); 
 					
 				}
-			} else SynErr(258);
+			} else SynErr(260);
 		}
 	}
 
@@ -4209,9 +4230,9 @@ List<Expression> decreases, ref Attributes decAttrs, ref Attributes modAttrs, st
 						RelationalExpression(out e1, allowSemi, allowLambda, allowBitwiseOps);
 						e0 = new BinaryExpr(x, BinaryExpr.Opcode.Or, e0, e1); 
 					}
-				} else SynErr(259);
+				} else SynErr(261);
 			}
-		} else SynErr(260);
+		} else SynErr(262);
 	}
 
 	void ImpliesExpression(out Expression e0, bool allowSemi, bool allowLambda, bool allowBitwiseOps) {
@@ -4331,7 +4352,7 @@ List<Expression> decreases, ref Attributes decAttrs, ref Attributes modAttrs, st
 				x = t;  op = BinaryExpr.Opcode.RightShift; 
 				Expect(79);
 				x.val = "<<";  Contract.Assert(t.pos == x.pos + 1); 
-			} else SynErr(261);
+			} else SynErr(263);
 			Term(out e1, allowSemi, allowLambda, allowBitwiseOps);
 			e0 = new BinaryExpr(x, op, e0, e1); 
 		}
@@ -4429,7 +4450,7 @@ List<Expression> decreases, ref Attributes decAttrs, ref Attributes modAttrs, st
 			x = t;  op = BinaryExpr.Opcode.Ge; 
 			break;
 		}
-		default: SynErr(262); break;
+		default: SynErr(264); break;
 		}
 	}
 
@@ -4461,7 +4482,7 @@ List<Expression> decreases, ref Attributes decAttrs, ref Attributes modAttrs, st
 		} else if (la.kind == 103) {
 			Get();
 			x = t;  op = BinaryExpr.Opcode.Sub; 
-		} else SynErr(263);
+		} else SynErr(265);
 	}
 
 	void BitvectorFactor(out Expression e0, bool allowSemi, bool allowLambda, bool allowBitwiseOps) {
@@ -4504,7 +4525,7 @@ List<Expression> decreases, ref Attributes decAttrs, ref Attributes modAttrs, st
 					AsExpression(out e1, allowSemi, allowLambda, allowBitwiseOps);
 					e0 = new BinaryExpr(x, op, e0, e1); 
 				}
-			} else SynErr(264);
+			} else SynErr(266);
 		}
 	}
 
@@ -4519,7 +4540,7 @@ List<Expression> decreases, ref Attributes decAttrs, ref Attributes modAttrs, st
 		} else if (la.kind == 142) {
 			Get();
 			x = t;  op = BinaryExpr.Opcode.Mod; 
-		} else SynErr(265);
+		} else SynErr(267);
 	}
 
 	void AsExpression(out Expression e, bool allowSemi, bool allowLambda, bool allowBitwiseOps) {
@@ -4590,7 +4611,7 @@ List<Expression> decreases, ref Attributes decAttrs, ref Attributes modAttrs, st
 			while (IsSuffix()) {
 				Suffix(ref e);
 			}
-		} else SynErr(266);
+		} else SynErr(268);
 	}
 
 	void MapDisplayExpr(IToken/*!*/ mapToken, bool finite, out Expression e) {
@@ -4644,13 +4665,13 @@ List<Expression> decreases, ref Attributes decAttrs, ref Attributes modAttrs, st
 				} else if (la.kind == 122) {
 					HashCall(id, out openParen, out typeArgs, out args);
 				} else if (StartOf(34)) {
-				} else SynErr(267);
+				} else SynErr(269);
 				e = new ExprDotName(id, e, id.val, typeArgs);
 				if (openParen != null) {
 				 e = new ApplySuffix(openParen, e, args);
 				}
 				
-			} else SynErr(268);
+			} else SynErr(270);
 		} else if (la.kind == 74) {
 			Get();
 			x = t; 
@@ -4698,7 +4719,7 @@ List<Expression> decreases, ref Attributes decAttrs, ref Attributes modAttrs, st
 						multipleIndices.Add(ee);
 						
 					}
-				} else SynErr(269);
+				} else SynErr(271);
 			} else if (la.kind == 153) {
 				Get();
 				anyDots = true; 
@@ -4706,7 +4727,7 @@ List<Expression> decreases, ref Attributes decAttrs, ref Attributes modAttrs, st
 					Expression(out ee, true, true);
 					e1 = ee; 
 				}
-			} else SynErr(270);
+			} else SynErr(272);
 			if (multipleIndices != null) {
 			 e = new MultiSelectExpr(x, e, multipleIndices);
 			 // make sure an array class with this dimensionality exists
@@ -4750,7 +4771,7 @@ List<Expression> decreases, ref Attributes decAttrs, ref Attributes modAttrs, st
 			}
 			Expect(77);
 			e = new ApplySuffix(openParen, e, args); 
-		} else SynErr(271);
+		} else SynErr(273);
 	}
 
 	void ISetDisplayExpr(IToken/*!*/ setToken, bool finite, out Expression e) {
@@ -4791,7 +4812,7 @@ List<Expression> decreases, ref Attributes decAttrs, ref Attributes modAttrs, st
 				}
 			}
 			Expect(77);
-		} else SynErr(272);
+		} else SynErr(274);
 		while (la.kind == 67 || la.kind == 68) {
 			if (la.kind == 67) {
 				Get();
@@ -4831,7 +4852,7 @@ List<Expression> decreases, ref Attributes decAttrs, ref Attributes modAttrs, st
 				isExistentialGuard = true; 
 			} else if (StartOf(9)) {
 				Expression(out e, true, true);
-			} else SynErr(273);
+			} else SynErr(275);
 			Expect(37);
 			Expression(out e0, true, true, true);
 			Expect(38);
@@ -4900,7 +4921,7 @@ List<Expression> decreases, ref Attributes decAttrs, ref Attributes modAttrs, st
 			NamedExpr(out e, allowSemi, allowLambda, allowBitwiseOps);
 			break;
 		}
-		default: SynErr(274); break;
+		default: SynErr(276); break;
 		}
 	}
 
@@ -4915,7 +4936,7 @@ List<Expression> decreases, ref Attributes decAttrs, ref Attributes modAttrs, st
 		} else if (la.kind == 122) {
 			HashCall(id, out openParen, out typeArgs, out args);
 		} else if (StartOf(34)) {
-		} else SynErr(275);
+		} else SynErr(277);
 		e = new NameSegment(id, id.val, typeArgs);
 		if (openParen != null) {
 		 e = new ApplySuffix(openParen, e, args);
@@ -4944,7 +4965,7 @@ List<Expression> decreases, ref Attributes decAttrs, ref Attributes modAttrs, st
 			}
 			e = new SeqDisplayExpr(x, elements); 
 			Expect(75);
-		} else SynErr(276);
+		} else SynErr(278);
 	}
 
 	void MultiSetExpr(out Expression e) {
@@ -4968,7 +4989,7 @@ List<Expression> decreases, ref Attributes decAttrs, ref Attributes modAttrs, st
 			Expression(out e, true, true);
 			e = new MultiSetFormingExpr(x, e); 
 			Expect(77);
-		} else SynErr(277);
+		} else SynErr(279);
 	}
 
 	void ConstAtomExpression(out Expression e, bool allowSemi, bool allowLambda) {
@@ -5089,7 +5110,7 @@ List<Expression> decreases, ref Attributes decAttrs, ref Attributes modAttrs, st
 			ParensExpression(out e, allowSemi, allowLambda);
 			break;
 		}
-		default: SynErr(278); break;
+		default: SynErr(280); break;
 		}
 	}
 
@@ -5118,7 +5139,7 @@ List<Expression> decreases, ref Attributes decAttrs, ref Attributes modAttrs, st
 			 n = BigInteger.Zero;
 			}
 			
-		} else SynErr(279);
+		} else SynErr(281);
 	}
 
 	void Dec(out Basetypes.BigDec d) {
@@ -5218,7 +5239,7 @@ List<Expression> decreases, ref Attributes decAttrs, ref Attributes modAttrs, st
 				CaseExpression(out c, allowSemi, allowLambda, allowBitwiseOps);
 				cases.Add(c); 
 			}
-		} else SynErr(280);
+		} else SynErr(282);
 		e = new MatchExpr(x, e, cases, usesOptionalBraces); 
 	}
 
@@ -5236,7 +5257,7 @@ List<Expression> decreases, ref Attributes decAttrs, ref Attributes modAttrs, st
 		} else if (la.kind == 139 || la.kind == 140) {
 			Exists();
 			x = t; 
-		} else SynErr(281);
+		} else SynErr(283);
 		QuantifierDomain(out bvars, out attrs, out range);
 		QSep();
 		Expression(out body, allowSemi, allowLambda);
@@ -5289,7 +5310,7 @@ List<Expression> decreases, ref Attributes decAttrs, ref Attributes modAttrs, st
 			AssumeStmt(out s);
 		} else if (la.kind == 35) {
 			CalcStmt(out s);
-		} else SynErr(282);
+		} else SynErr(284);
 	}
 
 	void LetExpr(out Expression e, bool allowSemi, bool allowLambda, bool allowBitwiseOps) {
@@ -5333,7 +5354,7 @@ List<Expression> decreases, ref Attributes decAttrs, ref Attributes modAttrs, st
 			 }
 			}
 			
-		} else SynErr(283);
+		} else SynErr(285);
 		Expression(out e, false, true);
 		letRHSs.Add(e); 
 		while (la.kind == 25) {
@@ -5395,7 +5416,7 @@ List<Expression> decreases, ref Attributes decAttrs, ref Attributes modAttrs, st
 				arguments.Add(pat); 
 			}
 			Expect(77);
-		} else SynErr(284);
+		} else SynErr(286);
 		Expect(33);
 		Expression(out body, allowSemi, allowLambda, allowBitwiseOps);
 		c = new MatchCaseExpr(x, name, arguments, body); 
@@ -5429,7 +5450,7 @@ List<Expression> decreases, ref Attributes decAttrs, ref Attributes modAttrs, st
 		} else if (la.kind == 2) {
 			Get();
 			id = t; 
-		} else SynErr(285);
+		} else SynErr(287);
 		Expect(97);
 		Expression(out e, true, true);
 	}
@@ -5706,95 +5727,97 @@ public class Errors {
 			case 194: s = "invalid IteratorSpec"; break;
 			case 195: s = "invalid Variance"; break;
 			case 196: s = "invalid TPCharOption"; break;
-			case 197: s = "invalid KType"; break;
-			case 198: s = "this symbol not expected in MethodSpec"; break;
-			case 199: s = "invalid MethodSpec"; break;
+			case 197: s = "invalid FuMe_Ident"; break;
+			case 198: s = "invalid KType"; break;
+			case 199: s = "this symbol not expected in MethodSpec"; break;
 			case 200: s = "invalid MethodSpec"; break;
-			case 201: s = "invalid FrameExpression"; break;
-			case 202: s = "this symbol not expected in FunctionSpec"; break;
-			case 203: s = "invalid FunctionSpec"; break;
-			case 204: s = "invalid PossiblyWildFrameExpression"; break;
-			case 205: s = "invalid PossiblyWildExpression"; break;
-			case 206: s = "this symbol not expected in OneStmt"; break;
-			case 207: s = "invalid OneStmt"; break;
+			case 201: s = "invalid MethodSpec"; break;
+			case 202: s = "invalid FrameExpression"; break;
+			case 203: s = "invalid TypeNameOrCtorSuffix"; break;
+			case 204: s = "this symbol not expected in FunctionSpec"; break;
+			case 205: s = "invalid FunctionSpec"; break;
+			case 206: s = "invalid PossiblyWildFrameExpression"; break;
+			case 207: s = "invalid PossiblyWildExpression"; break;
 			case 208: s = "this symbol not expected in OneStmt"; break;
 			case 209: s = "invalid OneStmt"; break;
-			case 210: s = "invalid AssertStmt"; break;
-			case 211: s = "invalid AssertStmt"; break;
-			case 212: s = "invalid AssumeStmt"; break;
-			case 213: s = "invalid UpdateStmt"; break;
-			case 214: s = "invalid UpdateStmt"; break;
-			case 215: s = "this symbol not expected in VarDeclStatement"; break;
-			case 216: s = "invalid VarDeclStatement"; break;
-			case 217: s = "invalid VarDeclStatement"; break;
-			case 218: s = "invalid IfStmt"; break;
-			case 219: s = "invalid IfStmt"; break;
-			case 220: s = "invalid WhileStmt"; break;
-			case 221: s = "invalid WhileStmt"; break;
-			case 222: s = "invalid MatchStmt"; break;
-			case 223: s = "invalid ForallStmt"; break;
-			case 224: s = "invalid ForallStmt"; break;
-			case 225: s = "invalid CalcStmt"; break;
-			case 226: s = "invalid ModifyStmt"; break;
-			case 227: s = "this symbol not expected in ModifyStmt"; break;
+			case 210: s = "this symbol not expected in OneStmt"; break;
+			case 211: s = "invalid OneStmt"; break;
+			case 212: s = "invalid AssertStmt"; break;
+			case 213: s = "invalid AssertStmt"; break;
+			case 214: s = "invalid AssumeStmt"; break;
+			case 215: s = "invalid UpdateStmt"; break;
+			case 216: s = "invalid UpdateStmt"; break;
+			case 217: s = "this symbol not expected in VarDeclStatement"; break;
+			case 218: s = "invalid VarDeclStatement"; break;
+			case 219: s = "invalid VarDeclStatement"; break;
+			case 220: s = "invalid IfStmt"; break;
+			case 221: s = "invalid IfStmt"; break;
+			case 222: s = "invalid WhileStmt"; break;
+			case 223: s = "invalid WhileStmt"; break;
+			case 224: s = "invalid MatchStmt"; break;
+			case 225: s = "invalid ForallStmt"; break;
+			case 226: s = "invalid ForallStmt"; break;
+			case 227: s = "invalid CalcStmt"; break;
 			case 228: s = "invalid ModifyStmt"; break;
-			case 229: s = "invalid LabelIdent"; break;
-			case 230: s = "invalid ReturnStmt"; break;
-			case 231: s = "invalid Rhs"; break;
-			case 232: s = "invalid Rhs"; break;
-			case 233: s = "invalid Lhs"; break;
-			case 234: s = "invalid NewArray"; break;
-			case 235: s = "invalid CasePattern"; break;
-			case 236: s = "invalid AlternativeBlock"; break;
-			case 237: s = "invalid Guard"; break;
-			case 238: s = "invalid AlternativeBlockCase"; break;
-			case 239: s = "this symbol not expected in AlternativeBlockCase"; break;
-			case 240: s = "this symbol not expected in AlternativeBlockCase"; break;
-			case 241: s = "this symbol not expected in LoopSpec"; break;
-			case 242: s = "this symbol not expected in LoopSpec"; break;
+			case 229: s = "this symbol not expected in ModifyStmt"; break;
+			case 230: s = "invalid ModifyStmt"; break;
+			case 231: s = "invalid LabelIdent"; break;
+			case 232: s = "invalid ReturnStmt"; break;
+			case 233: s = "invalid Rhs"; break;
+			case 234: s = "invalid Rhs"; break;
+			case 235: s = "invalid Lhs"; break;
+			case 236: s = "invalid NewArray"; break;
+			case 237: s = "invalid CasePattern"; break;
+			case 238: s = "invalid AlternativeBlock"; break;
+			case 239: s = "invalid Guard"; break;
+			case 240: s = "invalid AlternativeBlockCase"; break;
+			case 241: s = "this symbol not expected in AlternativeBlockCase"; break;
+			case 242: s = "this symbol not expected in AlternativeBlockCase"; break;
 			case 243: s = "this symbol not expected in LoopSpec"; break;
-			case 244: s = "invalid LoopSpec"; break;
-			case 245: s = "invalid CaseStatement"; break;
-			case 246: s = "this symbol not expected in CaseStatement"; break;
-			case 247: s = "this symbol not expected in CaseStatement"; break;
-			case 248: s = "invalid CalcOp"; break;
-			case 249: s = "invalid EquivOp"; break;
-			case 250: s = "invalid ImpliesOp"; break;
-			case 251: s = "invalid ExpliesOp"; break;
-			case 252: s = "invalid AndOp"; break;
-			case 253: s = "invalid OrOp"; break;
-			case 254: s = "invalid NegOp"; break;
-			case 255: s = "invalid Forall"; break;
-			case 256: s = "invalid Exists"; break;
-			case 257: s = "invalid QSep"; break;
-			case 258: s = "invalid ImpliesExpliesExpression"; break;
-			case 259: s = "invalid LogicalExpression"; break;
-			case 260: s = "invalid LogicalExpression"; break;
-			case 261: s = "invalid ShiftTerm"; break;
-			case 262: s = "invalid RelOp"; break;
-			case 263: s = "invalid AddOp"; break;
-			case 264: s = "invalid BitvectorFactor"; break;
-			case 265: s = "invalid MulOp"; break;
-			case 266: s = "invalid UnaryExpression"; break;
-			case 267: s = "invalid Suffix"; break;
-			case 268: s = "invalid Suffix"; break;
+			case 244: s = "this symbol not expected in LoopSpec"; break;
+			case 245: s = "this symbol not expected in LoopSpec"; break;
+			case 246: s = "invalid LoopSpec"; break;
+			case 247: s = "invalid CaseStatement"; break;
+			case 248: s = "this symbol not expected in CaseStatement"; break;
+			case 249: s = "this symbol not expected in CaseStatement"; break;
+			case 250: s = "invalid CalcOp"; break;
+			case 251: s = "invalid EquivOp"; break;
+			case 252: s = "invalid ImpliesOp"; break;
+			case 253: s = "invalid ExpliesOp"; break;
+			case 254: s = "invalid AndOp"; break;
+			case 255: s = "invalid OrOp"; break;
+			case 256: s = "invalid NegOp"; break;
+			case 257: s = "invalid Forall"; break;
+			case 258: s = "invalid Exists"; break;
+			case 259: s = "invalid QSep"; break;
+			case 260: s = "invalid ImpliesExpliesExpression"; break;
+			case 261: s = "invalid LogicalExpression"; break;
+			case 262: s = "invalid LogicalExpression"; break;
+			case 263: s = "invalid ShiftTerm"; break;
+			case 264: s = "invalid RelOp"; break;
+			case 265: s = "invalid AddOp"; break;
+			case 266: s = "invalid BitvectorFactor"; break;
+			case 267: s = "invalid MulOp"; break;
+			case 268: s = "invalid UnaryExpression"; break;
 			case 269: s = "invalid Suffix"; break;
 			case 270: s = "invalid Suffix"; break;
 			case 271: s = "invalid Suffix"; break;
-			case 272: s = "invalid LambdaExpression"; break;
-			case 273: s = "invalid EndlessExpression"; break;
-			case 274: s = "invalid EndlessExpression"; break;
-			case 275: s = "invalid NameSegment"; break;
-			case 276: s = "invalid DisplayExpr"; break;
-			case 277: s = "invalid MultiSetExpr"; break;
-			case 278: s = "invalid ConstAtomExpression"; break;
-			case 279: s = "invalid Nat"; break;
-			case 280: s = "invalid MatchExpression"; break;
-			case 281: s = "invalid QuantifierGuts"; break;
-			case 282: s = "invalid StmtInExpr"; break;
-			case 283: s = "invalid LetExpr"; break;
-			case 284: s = "invalid CaseExpression"; break;
-			case 285: s = "invalid MemberBindingUpdate"; break;
+			case 272: s = "invalid Suffix"; break;
+			case 273: s = "invalid Suffix"; break;
+			case 274: s = "invalid LambdaExpression"; break;
+			case 275: s = "invalid EndlessExpression"; break;
+			case 276: s = "invalid EndlessExpression"; break;
+			case 277: s = "invalid NameSegment"; break;
+			case 278: s = "invalid DisplayExpr"; break;
+			case 279: s = "invalid MultiSetExpr"; break;
+			case 280: s = "invalid ConstAtomExpression"; break;
+			case 281: s = "invalid Nat"; break;
+			case 282: s = "invalid MatchExpression"; break;
+			case 283: s = "invalid QuantifierGuts"; break;
+			case 284: s = "invalid StmtInExpr"; break;
+			case 285: s = "invalid LetExpr"; break;
+			case 286: s = "invalid CaseExpression"; break;
+			case 287: s = "invalid MemberBindingUpdate"; break;
 
       default: s = "error " + n; break;
     }
